Rake_gte.lean
@@ -1,0 +1,65 @@
+/-
+This was originally used in RakeSieve to provide the condition
+that the terms were all greater than or equal to 2. In the interest
+of time, I have left it unverified and moved it to this file.
+-/
+
+import Rake
+
+section gte_lemmas
+
+  variable (rm: RakeMap prop) (p n: Nat)
+
+  -- the gist of the argument I want to make here is that
+  -- for each k (sequence), I just fast-forward it so that
+  -- it skips over the discarded terms. we have these:
+  -- theorem gte_term (s : ASeq) (n : Nat) : s.d > 0 → n ≤ term (s.gte n) 0
+  -- theorem gte_same_delta (s : ASeq) (n : Nat) : (s.gte n).d = s.d
+  -- lemma Rake.___unused______ex_seq (r: Rake) : (r.term m = n) → (∃k ∈ r.ks, n = k + r.d * (m/r.ks.length))
+  -- we're /potentially/ modifying every single constant.
+  -- we have to say for each sequence:
+  --    - we drop only the terms we won't need
+  --    - we keep all the terms we used to have
+  --    - we don't add any new terms
+
+  lemma RakeMap.gte_drop -- gte drops terms < p
+    : n < p → ¬(∃m, (rm.rake.gte p).sort.val.term m = n) := by
+    -- why is this true? because `gte` removes all `k∈ks, k < p` and replaces them
+    -- with (d*x)+k... basically fast forwarding the sequence. but of course,
+    -- this only works if d is positive.
+    intro hnp; push_neg; intro m
+    let ⟨r,hrs⟩  := (rm.rake.gte p).sort
+    show r.term m ≠ n
+    suffices p ≤ r.term 0 by have := Rake.sorted_min_term_zero r hrs m; omega
+    obtain ⟨k,hk,i₀,hi₀⟩ := r.term_simp 0
+    have : k ∈ r.ks := by
+      have : i₀.val = 0 := by aesop
+      have := List.get_mem r.ks i₀.val i₀.prop
+      simp_all
+    sorry
+
+  lemma RakeMap.gte_keep -- gte keeps terms ≥ p
+    : n≥p ∧ (∃pm, rm.rake.term pm = n) → (∃m, (rm.rake.gte p).sort.val.term m = n) := sorry
+    -- why do I believe this?
+
+  lemma RakeMap.gte_same -- gte introduces no new terms
+    : (∃m, (rm.rake.gte p).sort.val.term m = n) → (∃pm, rm.rake.term pm = n) := by
+    sorry
+
+end gte_lemmas
+
+-- this proof is basically the same as for Rake.rem. only the
+-- lemmas above are different.
+def RakeMap.gte (prev : RakeMap prop) (p: Nat)
+  : RakeMap (λ n => prop n ∧ n ≥ p) :=
+  let rake := (prev.rake.gte p).sort
+  let proof := by
+    intro n; symm
+    let hm : Prop := (∃m, rake.val.term m = n)
+    let hpm : Prop := (∃pm, prev.rake.term pm = n )
+    have : prop n ↔ hpm := prev.hbij n
+    have : n<p → ¬hm := gte_drop prev p n
+    have : n≥p ∧ hpm → hm := gte_keep prev p n
+    have : hm → hpm := gte_same prev p n
+    by_cases n<p; all_goals aesop
+  { rake := rake, hbij := proof }
